\documentclass[titlepage,landscape]{seminar}
\usepackage{url}
\usepackage{graphicx}
\usepackage[pdftex]{color}
\usepackage{hyperref}
\usepackage{epstopdf}
\usepackage{slides}

\newcommand{\frack}{\frac{1}{k}}

\begin{document}

\myslide{
\begin{eqnarray*}
\mbox{Probability that both offspring are $A_1$} &=& p^2 \\
\mbox{Probability that one offspring is $A_1$ and one is $A_2$} &=& 2pq \\
\mbox{Probability that both offspring are $A_2$} &=& q^2
\end{eqnarray*}
\vfill
\begin{eqnarray*}
P(p'=1) &=& p^2  \\
P(p'=1/2) &=& 2pq \\
P(p'=0) &=& q^2 
\end{eqnarray*}
}

\myslide{
\begin{eqnarray*}
P(p_1=1|p_0) &=& p_0^2  \\
P(p_1=1/2|p_0) &=& 2p_0q_0 \\
P(p_1=0|p_0) &=& q_0^2  
\end{eqnarray*}
}

\myslide{
\begin{eqnarray*}
P(p_1=1|p_0) &=& p_0^2  \\
P(p_1=1/2|p_0) &=& 2p_0q_0 \\
P(p_1=0|p_0) &=& q_0^2  
\end{eqnarray*}
\vfil
\begin{eqnarray*}
P(p_2=1|p_1) &=& p_1^2 \\
P(p_2=1/2|p_1) &=& 2p_1q_1 \\
P(p_2=0|p_1) &=& q_1^2 
\end{eqnarray*}
}

\myslide{
\footnotesize
\begin{eqnarray*}
P(p_2=1|p_0) &=& P(p_2=1|p_1=1)P(p_1=1|p_0) + P(p_2=1|p_1=1/2)P(p_1=1/2|p_0) \\
             &=& (1)(p_0^2) + (1/4)(2p_0q_0) \\
             &=& p_0^2 + (1/2)p_0q_0 \\
P(p_2=1/2|p_0) &=& P(p_2=1/2|p_1=1/2)P(p_1=1/2|p_0) \\
               &=& (1/2)(2p_0q_0) \\
               &=& p_0q_0 \\
P(p_2=0|p_0) &=& P(p_2=0|p_1=0)P(p_1=0|p_0) + P(p_2=0|p_1=1/2)P(p_1=1/2|p_0) \\
             &=& (1)(q_0^2) + (1/4)(2p_0q_0) \\
             &=& q_0^2 + (1/2)p_0q_0 
\end{eqnarray*}
}

\myslide{
\begin{eqnarray*}
P(p_t=1|p_0) &=& p_0^2 + \left(1 - (1/2)^{t-1}\right)p_0q_0 \\
P(p_t=1/2|p_0) &=& p_0q_0(1/2)^{t-2} \\
P(p_t=0|p_0) &=& q_0^2 + \left(1 - (1/2)^{t-1}\right)p_0q_0
\end{eqnarray*}
}

\myslide{
\[
P(\hbox{$j$ $A_1$ in offspring $|$ $i$ $A_1$ in parents}) =
{2N \choose j}\left(\frac{i}{2N}\right)\left(1 - \frac{i}{2N}\right)
\]
\vfil
\[
\hbox{Var}(p_{t+1}) = \frac{p_t(1-p_t)}{2N}
\]
}

\myslide{
\begin{eqnarray*}
f_{t+1} &=& \mbox{Prob. ibd from preceding generation} \\
        &&  + (\mbox{Prob. not ibd from prec. gen.}) \times (\mbox{Prob. ibd from
          earlier gen.}) \\
   &=& \frac{1}{2N} + \left(1 - \frac{1}{2N}\right)f_t
\end{eqnarray*}
\vfil
\[
f_{t+1} = 1 - \left(1 - \frac{1}{2N}\right)^t(1-f_0)
\]
}

\myslide{
\[
Var(p_{t+1}) = \frac{p_t(1-p_t)}{2N} \quad.
\]
\vfil
\[
N_e^{(v)} = \frac{p(1-p)}{2\widehat{Var}(p)}
\]
}

\myslide{
\[
f_{t+1}
   = \frac{1}{2N} + \left(1 - \frac{1}{2N}\right)f_t
\]
\vfil
\[
N_e^{(f)} = \frac{1 - \hat f_t}{2(\hat f_{t+1} - \hat f_t)}
\]
\vfil
Assume $\hat f_t = 0$
\[
N_e^{(f)} = \frac{1}{2\hat f_{t+1}}
\]
}

\end{document}

